added refinement theorem

src/Renaming.v
@@ -1,4 +1,5 @@
 Require Import Lib.FMap Lib.Struct Semantics Syntax String List.
+Require Import Program.Equality.
 
 Set Implicit Arguments.
 Section FnInv.
@@ -39,37 +40,98 @@ Section FnInv.
   Qed.
 End FnInv.
 
-Section AlphaRename.
-  Variable nameMap: string -> string.
-  Variable nameMap1To1: forall x y, nameMap x = nameMap y -> x = y.
-  Variable nameMapOnto: forall x, exists y, nameMap y = x.
+Section Rename.
+  Variable p: string -> string.
+  Variable p1To1: forall x y, p x = p y -> x = y.
+  Variable pOnto: forall x, exists y, p y = x.
 
-  Definition mapName A a := {| attrName := nameMap (@attrName A a); attrType := attrType a |}.
+  Definition mapNameAttr A a := {| attrName := p (@attrName A a); attrType := attrType a |}.
   
-  Fixpoint mapNames A (ls: list (Attribute A)) :=
-    map (@mapName _) ls.
+  Fixpoint mapNamesList A (ls: list (Attribute A)) :=
+    map (@mapNameAttr _) ls.
 
   Definition mapNamesMap A (m: M.t A) :=
-    M.fold (fun k v old => M.add (nameMap k) v old) m (M.empty _).
+    M.fold (fun k v old => M.add (p k) v old) m (M.empty _).
 
   Lemma mapNamesMapEmpty A: mapNamesMap (M.empty A) = M.empty A.
   Proof.
     apply (M.F.P.fold_Empty); intuition.
   Qed.
 
+  Lemma mapNamesMapAdd A m: forall k (v: A),
+      ~ M.In k m ->
+      mapNamesMap (M.add k v m) = M.add (p k) v (mapNamesMap m).
+  Proof.
+    intros; unfold mapNamesMap; rewrite M.F.P.fold_add; simpl in *; intuition.
+    unfold M.F.P.transpose_neqkey; intros.
+    assert (pneq: p k0 <> p k') by (unfold not; intros; apply H0; apply p1To1; intuition).
+    apply M.transpose_neqkey_eq_add; intuition.
+  Qed.
+  
+  Lemma mapNamesMapsTo1 A m: forall k (v: A),
+      M.MapsTo k v m ->
+      M.MapsTo (p k) v (mapNamesMap m).
+  Proof.
+    M.mind m.
+    - apply M.F.P.F.empty_mapsto_iff in H; intuition.
+    - apply M.F.P.F.add_mapsto_iff in H1.
+      destruct H1 as [[keq veq] | [kneq kin]].
+      + subst.
+        rewrite mapNamesMapAdd; intuition.
+        apply M.F.P.F.add_mapsto_iff; intuition.
+      + specialize (H _ _ kin).
+        rewrite mapNamesMapAdd; intuition.
+        apply M.F.P.F.add_mapsto_iff; intuition.
+  Qed.
+
+  Lemma mapNamesMapsTo2 A m: forall k (v: A),
+      M.MapsTo (p k) v (mapNamesMap m) ->
+      M.MapsTo k v m.
+  Proof.
+    M.mind m.
+    - apply M.F.P.F.empty_mapsto_iff in H; intuition.
+    - rewrite mapNamesMapAdd in H1; intuition; apply M.F.P.F.add_mapsto_iff in H1.
+      destruct H1 as [[keq veq] | [kneq kin]].
+      + specialize (p1To1 keq).
+        subst.
+        apply M.F.P.F.add_mapsto_iff; intuition.
+      + specialize (H _ _ kin).
+        assert (kneq': k <> k0) by (unfold not; intros; subst; intuition).
+        apply M.F.P.F.add_mapsto_iff; intuition.
+  Qed.
+
   Definition mapNameUnitLabel l :=
     match l with
       | Rle None => Rle None
       | Meth None => Meth None
-      | Rle (Some r) => Rle (Some (nameMap r))
-      | Meth (Some {| attrName := f; attrType := v |}) => Meth (Some {| attrName := nameMap f; attrType := v |})
+      | Rle (Some r) => Rle (Some (p r))
+      | Meth (Some {| attrName := f; attrType := v |}) => Meth (Some {| attrName := p f; attrType := v |})
     end.
 
+  Section SomeType.
+    
+    Fixpoint mapNamesAction t k (a: ActionT t k) :=
+      match a with
+      | MCall meth s e cont => MCall (p meth) s e (fun v => mapNamesAction (cont v))
+      | Let_ lret' e cont => Let_ e (fun v => mapNamesAction (cont v))
+      | ReadReg r k cont => ReadReg r k (fun v => mapNamesAction (cont v))
+      | WriteReg r k e cont => WriteReg r e (mapNamesAction cont)
+      | IfElse e k t f cont => IfElse e (mapNamesAction t) (mapNamesAction f)
+                                      (fun v => mapNamesAction (cont v))
+      | Assert_ e cont => Assert_ e (mapNamesAction cont)
+      | Return e => Return e
+      end.
+
+    Lemma actionMapName o k a u cs r (sa: @SemAction o k a u cs r):
+      SemAction (mapNamesMap o) (mapNamesAction a) (mapNamesMap u) (mapNamesMap cs) r.
+    Proof.
+      dependent induction sa; simpl in *.
+      - 
   Lemma mapNamesKeysEq A (m: M.t A) l:
     M.KeysEq m l ->
-    M.KeysEq (mapNamesMap m) (map nameMap l).
+    M.KeysEq (mapNamesMap m) (map p l).
   Proof.
     admit.
   Qed.
 
-End AlphaRename.
+End Rename.
