src/Refinement.v
@@ -1,0 +1,61 @@
+Require Import Syntax Semantics String Lib.FMap Program.Equality List.
+
+Set Implicit Arguments.
+
+Section StepToRefinement.
+  Variable imp spec: Modules.
+  Variable p: MethsT -> MethsT.
+  Variable ruleMap: RegsT -> string -> option string.
+  Variable theta: RegsT -> RegsT.
+  Variable thetaInit: theta (initRegs (getRegInits imp)) = initRegs (getRegInits spec).
+
+  Definition liftPLabel o l :=
+    match l with
+    | {| annot := a; defs := dfs; calls := clls |} =>
+      {| annot := match a with
+                  | Some (Some r) => Some (ruleMap o r)
+                  | Some None => Some None
+                  | None => None
+                  end;
+         defs := p dfs;
+         calls := p clls |}
+    end.
+
+  Variable stepMap:
+    forall o u l, Step imp o u l ->
+             exists uspec, Step spec (theta o) uspec (liftPLabel o l) /\
+                      theta (M.union u o) = M.union uspec (theta o).
+
+  Theorem stepRefinement':
+    forall s sig, Behavior imp s sig ->
+                  exists sigSpec, Behavior spec (theta s) sigSpec /\
+                                  equivalentLabelSeq p sig sigSpec.
+  Proof.
+    intros.
+    dependent induction H.
+    dependent induction HMultistepBeh; subst.
+    - exists nil; rewrite thetaInit; repeat constructor.
+    - specialize (IHHMultistepBeh thetaInit stepMap eq_refl).
+      pose proof (stepMap HStep) as [uSpec [stepSpec upd]].
+      destruct IHHMultistepBeh as [sigSpec [behSpec eqv]].
+      inversion behSpec; subst.
+      pose proof (BehaviorIntro (Multi HMultistepBeh0 stepSpec)) as sth.
+      rewrite <- upd in sth.
+      exists (liftPLabel n l :: sigSpec).
+      constructor.
+      + intuition.
+      + constructor.
+        * unfold equivalentLabel, liftPLabel; simpl.
+          destruct l; destruct annot; simpl; intuition.
+          destruct o; simpl; intuition.
+        * intuition.
+  Qed.
+
+  Theorem stepRefinement: traceRefines p imp spec.
+  Proof.
+    unfold traceRefines; intros.
+    pose proof (stepRefinement' H) as [sigSpec beh].
+    exists (theta s1); exists sigSpec.
+    intuition.
+  Qed.
+End StepToRefinement.
